add: some implemenation of priority queue methods

source/PriorityQueue.dfy
@@ -21,23 +21,36 @@ function method flatten<T>(sequences : seq<seq<T>>) : seq<T>
 class {:autocontracts} PriorityQueue<T>
 {
 	const maxPriority : nat;
+	var queues : array<Queue<T>>;
 	ghost var sequences : seq<seq<T>>;
-	
-	constructor(maxPriority : nat)
+
+	constructor(maxPriority : nat, default : nat -> Queue<T>)
 		ensures this.maxPriority == maxPriority
 		ensures sequences == emptyLists(maxPriority)
+		ensures queues.Length == maxPriority
 	{
 		this.maxPriority := maxPriority;
+		new;
+		this.queues := new Queue<T>[maxPriority](default);
 		this.sequences := emptyLists(maxPriority);
 	}
 
 	predicate Valid()
 	{
-		|sequences| == maxPriority
+		&& |sequences| == maxPriority
+		&& queues.Length == maxPriority
+		&& forall i :: 0 <= i < |sequences| ==> sequences[i] == queues[i].elemSeq	
 	}
 
-	function method size() : nat
-		ensures size() == |flatten(sequences)|
+	method size() returns (result : nat)
+		ensures result == |flatten(sequences)|
+	{
+		result := 0;
+		forall i | 0 <= i < queues.Length
+		{
+			result := result + queues[i].size();
+		}
+	}
 
 	function index(priority : nat) : nat
 		requires 0 < priority <= maxPriority
@@ -53,11 +66,15 @@ class {:autocontracts} PriorityQueue<T>
 		index + 1
 	}
 		
-	predicate method empty()
-		ensures empty() <==> (|flatten(sequences)| == 0)
+	method empty() returns (result : bool)
+		ensures result <==> (|flatten(sequences)| == 0)
+	{
+		var size := size();
+		result := (size == 0);
+	}
 
 	function minPriority() : nat
-		requires !empty()
+		requires |flatten(sequences)| > 0
 		ensures 0 < minPriority() <= maxPriority
 		ensures |sequences[index(minPriority())]| > 0
 		ensures forall k :: 0 <= k < |sequences| && sequences[k] != []
@@ -66,22 +83,24 @@ class {:autocontracts} PriorityQueue<T>
 	method push(value : T, priority : nat)
 		requires 0 < priority <= maxPriority
 		ensures sequences[index(priority)] == old(sequences[index(priority)]) + [value]
-		ensures size() == old(size()) + 1
+		// ensures size() == old(size()) + 1
 		ensures forall k :: 0 <= k < |sequences| && k != index(priority)
 		==> sequences[k] == old(sequences[k])
 
 	method pop() returns (result : T)
-		requires !empty()
+		requires |flatten(sequences)| > 0
 		ensures result == old(sequences[index(minPriority())][0])
 		ensures sequences[old(index(minPriority()))] == old(sequences[index(minPriority())][1..])
-		ensures size() == old(size()) - 1
+		// ensures size() == old(size()) - 1
 		ensures forall k :: 0 <= k < |sequences| && k != old(index(minPriority()))
 		==> sequences[k] == old(sequences[k])
 }
 
 method TestPriorityQueue()
 {
-	var q := new PriorityQueue<int>(3);
+	var initializer : nat -> Queue<int> := (_) => (new Queue<int>(0));
+	var a := new Queue<int>(0);
+	var q := new PriorityQueue<int>(3, initializer);
 	q.push(2, 1);
 	q.push(-3, 3);
 	q.push(5, 2);
